ZFMetaRec.thy
@@ -19,9 +19,9 @@ ML {*
   fun tracing_proc ctxt (ct, _, _) =
     let
       val thy = Proof_Context.theory_of ctxt
-      val ruletrace = MetaRec.get_rule_trace ctxt |> map (fn f => f ())
-      val _ = tracing (Syntax.string_of_term ctxt (Thm.term_of ct)^"\nrule trace:\n"
-        ^cat_lines (map (Syntax.string_of_term ctxt) ruletrace))
+      val _ = tracing (MetaRec.compose_err_from_trace ctxt
+        ("\n\ntracing "^Syntax.string_of_term ctxt (Thm.term_of ct))
+        ^"\n\n")
       val th = Drule.instantiate' [SOME (Thm.ctyp_of_term ct)] [SOME ct] @{thm tracingI}
     in
       (th, [])
@@ -33,12 +33,12 @@ setup {*
 *}
 
 definition
-  fail_const where
-  [MRjud 1 0]: "fail_const(x) == False"
+  fail_const where (* FOL's false not general enough in all cases *)
+  [MRjud 1 0]: "fail_const(x) == (!! P::prop. PROP P)"
 
 abbreviation
-  fail :: "o" where
-  "fail == fail_const(0)"
+  fail_abbrev :: "prop" ("fail") where
+  "fail_abbrev == fail_const(0)"
 
 
 
@@ -96,84 +96,385 @@ ML {*
     |> the_default t
 
 
-  fun metaexs_to_freshvars t ctxt =
+  fun metaexs_to_freshvars lift_fixes t ctxt =
     case try dest_metaex t of
       SOME (x, T, body) => 
         let
-          val (v, ctxt2) = MetaRec.genvar_on_run_state x T ctxt
-          val body' = Term.subst_bound (v, body)
+          val (v, ctxt2) = MetaRec.genvar_on_run_state x (map fastype_of lift_fixes ---> T) ctxt
+          val body' = Term.subst_bound (list_comb (v, lift_fixes), body)
         in
-          metaexs_to_freshvars body' ctxt2
+          metaexs_to_freshvars lift_fixes body' ctxt2
         end
     | _ => (t, ctxt)
 *}
 
 ML {*
+  
+  fun aconv_norm ctxt_ = MetaRec.aconv_norm (MetaRec.norm_with_env_in_run_state ctxt_)
 
+
+  (* TODO(opt!): use exact_net for memo_net and constraint_to_pats
+     (instantiated pats should then continue to work memoized -> use aconv_norm insteaf aconv comparisons) *)
   structure ExConstraintMemoization = Proof_Data(
-      (* ex_constraint results are indexed by their search pattern terms,
-         which are converted to fully-dest_metaex'd *open* terms *)
-      type T = (term * term) Net.net
-      fun init _ = Net.empty
+      (* ex_constraint results are indexed in memo_net by their search pattern terms,
+           which are converted to fully-dest_metaex'd *open* terms.
+         constraint_to_pats maps an active constraint to the patterns that have
+           been matched against it (as (C, pat) entries in net that differ in pat).
+         fix_necessary_tab says which memoized pattern results depend on a metarec fix. *)
+      type T = { memo_net: (term * (term * term)) Net.net,
+        constraint_to_pats: (term * term) Net.net,
+        fix_necessary_tab: term list Symtab.table }
+      fun init _ = { memo_net = Net.empty, constraint_to_pats = Net.empty,
+        fix_necessary_tab = Symtab.empty }
     );
 
-  (* memoization table is reset on every linear context boundary,
-     esp. after each constraint simplification phase *)
-  fun ex_constraint_memo_linctxt_boundary_handler _ = ExConstraintMemoization.map (K Net.empty)
 
-  (* TODO(feature): support for matching constraints from nontrivial local context
-     -> lifting of unifvars in pat_vard over quantifications of C and matching against
-        C's conclusion? Do we also have to spell these quantifications out in pat? *)
-  (* TODO(feature): further filtering of matching constraints via metarec judgement *)
+  (* NB: pat_indexing contains loose bounds for metaex quantified vars and refers
+       to the concrete local_frees, i.e. no lifting here *)
+  val calc_pat_indexing = fully_dest_metaex #> Envir.eta_contract
+
+  (* NB: memoization for a constraint pattern is removed if a
+     relevant part of the metarec context is discharged (does not matter for foconstraints).
+     Memoization table is reset on every linear context boundary outside a metarec derivation,
+     esp. after each constraint simplification phase *)
+  fun ex_constraint_memo_linctxt_boundary_handler boundary ctxt linctxt =
+    let
+      fun del_pat pat memo_net = 
+        Net.delete_term (fn (pat, (pat2, _)) => pat aconv pat2)
+          (calc_pat_indexing pat, pat) memo_net
+      fun del_C safe C constraint_to_pats = 
+        (if safe then Net.delete_term_safe else Net.delete_term)
+          (fn (C, (C2, _)) => aconv_norm ctxt (C, C2))
+          (Envir.eta_contract (MetaRec.norm_with_env_in_run_state ctxt C), C) constraint_to_pats
+      fun del_fixes_of pat fix_necessary_tab =
+        let val fixes = Term.add_frees pat [] |> map fst |> filter (Symtab.defined fix_necessary_tab)
+        in fix_necessary_tab |> fold (fn p => Symtab.remove_list (op aconv) (p, pat)) fixes end
+    in
+      linctxt |> ExConstraintMemoization.map (fn {memo_net, constraint_to_pats, fix_necessary_tab} =>
+        case boundary of
+          MetaRec.MetaRecCtxtDischargedBoundary disch_params =>
+            let 
+              val stale_pats = disch_params |> maps (Symtab.lookup fix_necessary_tab #> these)
+              val stale_Cs = stale_pats |> maps (fn stale_pat =>
+                Net.lookup memo_net (Net.key_of_term (calc_pat_indexing stale_pat))
+                |> filter (fn (pat, _) => stale_pat aconv pat) |> map (snd #> snd))
+            in
+              { memo_net = memo_net |> fold (fn stale_pat => fn net =>
+                    del_pat stale_pat net
+                    handle Net.DELETE => error ("ex_constraint_memo_linctxt_boundary_handler: internal error:"
+                      ^" pattern "^Syntax.string_of_term linctxt stale_pat
+                      ^" became stale now due to discharge of params "^commas disch_params
+                      ^", but not found in memoization net\n"
+                      ^(cat_lines (Net.content memo_net |> map (fn (_, (pat, C)) =>
+                          Syntax.string_of_term linctxt pat ^" -> "^Syntax.string_of_term linctxt C)))))
+                  stale_pats,
+                constraint_to_pats = constraint_to_pats |> fold (del_C false) stale_Cs
+                  handle Net.DELETE => error ("ex_constraint_memo_linctxt_boundary_handler: internal error:"
+                    ^" deletion of stale constraints "
+                    ^commas (stale_Cs |> map (MetaRec.str_of_normed_term ctxt))^" failed"),
+                fix_necessary_tab = fix_necessary_tab |> fold del_fixes_of stale_pats }
+             end
+        | MetaRec.MetaRecConstraintSimpBoundary simpd_C =>
+            (* NB: we remove simplified constraints from memo_net, so that ex_constraint result function
+               can expect a simplified constraint even in the memoized case *)
+            let val stale_pats = Net.match_term constraint_to_pats simpd_C
+              |> filter (fn (C, _) => aconv_norm ctxt (C, simpd_C)) |> map snd
+            in
+              { memo_net = memo_net |> fold del_pat stale_pats
+                  handle Net.DELETE => error ("ex_constraint_memo_linctxt_boundary_handler"
+                    ^" on MetaRecConstraintSimpBoundary "^MetaRec.str_of_normed_term ctxt simpd_C
+                    ^": del_pat failed."
+                    ^" stale_pats are "^commas (stale_pats |> map (MetaRec.str_of_normed_term ctxt))),
+                constraint_to_pats = constraint_to_pats |> del_C true simpd_C,
+                fix_necessary_tab = fix_necessary_tab |> fold del_fixes_of stale_pats }
+            end
+        | _ =>
+            { memo_net = Net.empty, constraint_to_pats = Net.empty,
+              fix_necessary_tab = Symtab.empty })
+    end
+
+
+  local
+    fun mk_env (tyenv, tenv) = Envir.Envir { maxidx = 0, tyenv=tyenv, tenv=tenv }
+    fun dest_env (Envir.Envir {tyenv, tenv, ...}) = (tyenv, tenv)
+    fun map_env f = mk_env o f o dest_env
+  in
+
+
+  (* TODO(opt!!): manage constraints in net/item_net for fast constraint matching.
+       (constraints cannot be stored with fixed unification variables in net because they
+         can become instantiated in the meantime) *)
+  (* TODO(feature):
+       * further filtering of matching constraints via metarec judgement
+       * multiple simultaneous left-to-right matchings by use of meta-conjunctions under meta-exists
+         (akin to matching the heads of a CHR or frule) *)
   fun ex_constraint_proc ctxt fail_cont (pat0, _, _) =
     let
+      val ctxt = MetaRec.metarec_simp_instantiated_constraints ctxt
+
       val thy = Proof_Context.theory_of ctxt
       val linctxt = MetaRec.get_linear_ctxt_in_run_state ctxt 
-      val memo_net = ExConstraintMemoization.get linctxt
+      val { memo_net, ... } = ExConstraintMemoization.get linctxt
 
+      (* NB: norming necessary in particular, because pattern_match_envctxt only norms object *)
       val pat = MetaRec.norm_with_env_in_run_state ctxt pat0
-      val pat_indexing = pat |> fully_dest_metaex |> Envir.eta_contract
-      fun aconv_norm ctxt_ = MetaRec.aconv_norm (MetaRec.norm_with_env_in_run_state ctxt_)
+      val assms = MetaRec.get_assms (Context.Proof ctxt) |> rev |> map (MetaRec.norm_with_env_in_run_state ctxt)
+      val (local_frees, rel_assms) = MetaRec.rel_frees_and_assms_of (K ()) ctxt pat
 
-      fun result pat_inst ctxt_ = 
+      (* val _ = tracing (MetaRec.compose_err_from_trace ctxt
+        ("\n\nex_constraint_proc on "^Syntax.string_of_term ctxt pat
+        ^"\n  local_frees are "^commas (local_frees |> map (Syntax.string_of_term ctxt))
+        ^"\n  rel_assms are "^commas (rel_assms |> map (Syntax.string_of_term ctxt))
+        ^"\n  assms are "^commas (assms |> map (Syntax.string_of_term ctxt)))
+        ^"\n\n") *)
+
+      val pat_indexing = pat |> calc_pat_indexing
+
+
+      fun result pat_inst0 C ctxt_ = 
         let
-          val C_prf = MetaRec.assumption_prf pat_inst
+          (* val _ = tracing ("ex_constraint_proc: in result proof construction for "
+            ^MetaRec.str_of_normed_term ctxt_ pat_inst0
+            ^"\nfrom constraint "^MetaRec.str_of_normed_term ctxt_ C) *)
+
+          val (pat_inst, C_normed) = (pat_inst0, C)
+            |> pairself (MetaRec.norm_with_env_in_run_state ctxt_)
+          val C_prf = MetaRec.assumption_prf C_normed
+
+          val pat_inst_prf = 
+            if C_normed aconv (pat_inst |> curry Logic.list_implies rel_assms |> fold_rev Logic.all local_frees) then
+              (* TODO(refactor): this proof construction is shared exactly with MetaRec.constraint_gen_proc *)
+              C_prf
+              |> fold (MetaRec.allE_rev_prf ctxt_) local_frees
+              |> fold (MetaRec.mp_rev_prf ctxt_ o MetaRec.assumption_prf) rel_assms
+            else (* find rotation of parameters of constraint and assumption matching *)
+              let
+                (* NB: we use matching modulo eta and eta-contract because instantiations
+                     of unification variables often lead to eta-redexes in constraint conclusions *)
+                (* TODO(correctness): seems unnecessary with on-the-fly simplification of instantiated constraints
+                   (which are then removed from memo_net) *)
+                val C_norm_cv = Thm.eta_conversion
+
+                val (C_normed_eta, pat_inst_eta) = (C_normed, pat_inst)
+                  |> pairself (MetaRec.term_cv ctxt C_norm_cv)
+                (* fixing unifvars in C that are not shared with pat *)
+                (* NB: freezing wrt. pat is not enough for assumption matching,
+                       because the constraint can further contain unification variables *)
+                val (([C', pat_inst_eta_frozen], ((freeze, _), (thaw, _))), ctxt_2) = ctxt_
+                  |> MetaRec.exact_freeze_thaw [C_normed_eta, pat_inst_eta]
+
+                (* fixing and then varifying parameters of fixed constraint *)
+                val ((fixing, C'_body), ctxt_3) = ctxt_2 |> Variable.focus C'
+                val (C'_assms, C'_concl) = Logic.strip_horn C'_body
+                val fix_frees = map (Free o snd) fixing
+                val [[C'_concl_fixvard], C'_assms_fixvard, fix_vars] = [[C'_concl], C'_assms, fix_frees]
+                  |> burrow (Variable.export_terms ctxt_3 ctxt_2)
+
+                (* val _ = tracing ("ex_constraint_proc: after fixvaring."
+                  ^"\n  fix_vars are "^commas (fix_vars |> map (Syntax.string_of_term ctxt_))
+                  ^"\n  fixvard concl is "^Syntax.string_of_term ctxt_ C'_concl_fixvard
+                  ^"\n  fixvard assms are "^commas (C'_assms_fixvard |> map (Syntax.string_of_term ctxt_))) *)
+
+                val thy = Proof_Context.theory_of ctxt_
+
+                (* matching local_frees against generalized focus frees. other unifvars are frozen *)
+                val env = (Vartab.empty, Vartab.empty)
+                  |> Pattern.match thy (C'_concl_fixvard, pat_inst_eta_frozen)
+                  |> mk_env
+                  handle Pattern.MATCH =>
+                      MetaRec.err_with_trace ctxt_3 ("ex_constraint_proc: frozen pat_inst "
+                        ^Syntax.string_of_term ctxt_3 pat_inst_eta_frozen
+                        ^" does not match completely frozen constraint with varified parameters "
+                        ^Syntax.string_of_term ctxt_3 C'_concl_fixvard)
+                    | Pattern.Pattern =>
+                      MetaRec.err_with_trace ctxt_3 "ex_constraint_proc: internal error: non-pattern in conclusion match"
+
+                (* val _ = tracing ("ex_constraint_proc: after matching. env is\n  "
+                  ^commas (env |> Envir.term_env |> Vartab.dest |> map (fn (ixn, (T, t)) =>
+                    Syntax.string_of_term ctxt_ (Var (ixn, T)) ^" := "^Syntax.string_of_term ctxt_ t))) *)
+
+                (* FIXME: use factual consequences as well. Seems necessary so that deep synthty derivations
+                    have corresponding x elabto x : A facts available.
+                    Problematic because non-ground facts are only availabe as rules, cf. fact constraint completion
+                    in constraint simplification, so this kills performance. *)
+                val frozen_assms = assms |> map freeze
+                val open_C'_assms = C'_assms_fixvard |> map (Envir.norm_term env)
+                  |> subtract (op aconv) frozen_assms
+
+                (* val _ = tracing ("ex_constraint_proc: after calculation of open assumptions") *)
+
+                (* minor FIXME: backtracking over previous match-choices *)
+                val env2 = env |> fold (fn open_C'_assm => fn env_ =>
+                    case get_first (fn rel_assm =>
+                        try (map_env (Pattern.match thy (open_C'_assm, rel_assm))) env_)
+                      frozen_assms
+                    of
+                      SOME env_2 => env_2
+                    | NONE =>
+                        MetaRec.err_with_trace ctxt_ ("ex_constraint_proc: found constraint "^Syntax.string_of_term ctxt_ C'
+                        ^" matching "^Syntax.string_of_term ctxt_ pat
+                        ^"\nbut the constraint assumptions "^Syntax.string_of_term ctxt_ open_C'_assm
+                        ^"\nare has no match in assms "^commas (assms |> map (Syntax.string_of_term ctxt_))))
+                  open_C'_assms
+
+                (* val _ = tracing ("ex_constraint_proc: after assumption matching. env2 is "
+                  ^commas (env2 |> Envir.term_env |> Vartab.dest |> map (fn (ixn, (T, t)) =>
+                    Syntax.string_of_term ctxt_ (Var (ixn, T)) ^" := "^Syntax.string_of_term ctxt_ t))) *)
+
+              in
+                C_prf
+                |> MetaRec.conv_prf ctxt_ C_norm_cv
+                |> fold (MetaRec.allE_rev_prf ctxt_ o thaw o Envir.norm_term env2) fix_vars
+                |> fold (MetaRec.mp_rev_prf ctxt_ o MetaRec.assumption_prf o thaw o Envir.norm_term env2)
+                     C'_assms_fixvard
+                |> MetaRec.unconvd_from_prf ctxt_ C_norm_cv pat_inst
+              end
+
           val (inst_intro, ctxt_2) = MetaRec.inst_match_on_freshthm_prf
             @{thm ex_constraintI} [NONE, SOME pat] ctxt_
-          val (res_prf, ctxt_3) = MetaRec.mps_match_prf inst_intro [C_prf] ctxt_2
+          val (res_prf, ctxt_3) = MetaRec.mps_match_prf inst_intro [pat_inst_prf] ctxt_2
+
+          (* val _ = tracing ("ex_constraint_proc: result proof construction done for "
+            ^MetaRec.str_of_normed_term ctxt_3 (MetaRec.prop_of_proofp res_prf)) *)
         in
-          ((res_prf, [pat_inst]), SOME (ctxt_3 |> Context.Proof |> MetaRec.get_the_run_state))
+          ((res_prf, [pat_inst]), ctxt_3 |> Context.Proof |> MetaRec.get_the_run_state |> SOME)
         end
     in
       case Net.match_term memo_net pat_indexing |> filter (fn (pat2, _) => aconv_norm ctxt (pat2, pat)) of
-        (_, pat_inst) :: _ => result pat_inst ctxt
+        (_, (pat_inst, C)) :: _ =>
+          result pat_inst C ctxt
       | [] =>
           let
-            val constraints = MetaRec.get_constraints_in_run_state ctxt
+            val constraints = MetaRec.get_active_constraints_in_run_state ctxt
+            val (([pat_fxd], ((freeze, _), (thaw, _))), ctxt2) = MetaRec.exact_freeze_thaw [pat] ctxt
+
             (* NB: we don't use Variable.import/export because they are not proper inverses due to
                  re-maxidx-ification of unification variable names *)
-            val (([pat_fxd], ((freeze, _), (thaw, _))), ctxt2) = MetaRec.exact_freeze_thaw [pat] ctxt
-            val (pat_fxd_vard, ctxt3) = ctxt2 |> metaexs_to_freshvars pat_fxd
+            val ((pat_fxd_liftvard, pat_fxd_vard), ctxt3) = ctxt2
+              |> metaexs_to_freshvars local_frees pat_fxd
+              ||>> metaexs_to_freshvars [] pat_fxd
+
+           (* NB: since assumptions are constant in one context extension level,
+               we only match lifted constraint conclusion.
+               We don't have to care about the case of further instantiation of unification variables
+               in particular, because their dependencies already have to be present. *)
+            val pat_fxd_vard_lifted = pat_fxd_liftvard |> fold_rev Logic.all local_frees
+            val [[pat_fxd_vard_fixvard], fixvars] = [[pat_fxd_vard], local_frees]
+              |> burrow (map (Term_Subst.generalize ([], map (Term.dest_Free #> fst) local_frees)
+                   (Term.maxidx_of_term pat_fxd_vard)))
+            val fixvar_to_local_free = fixvars ~~ local_frees
+
+            fun prep_match mod_param_rot C =
+              let
+                (* NB: object is normed by pattern_match_envctxt, but freezing interferes *)
+                val C' = C |> MetaRec.norm_with_env_in_run_state ctxt3 |> freeze
+                val ((fixing, C''), ctxt_) = Variable.focus C' ctxt3
+                val fix_frees = fixing |> map snd
+                val concl = Logic.strip_assums_concl C''
+                val rel_fixes = fix_frees |> inter (op =) (Term.add_frees concl [])
+              in
+                if mod_param_rot then concl
+                else fold_rev (Logic.all o Free) rel_fixes concl
+              end
+
+            (* val _ = tracing ("ex_constraint_proc: searching a constraint matching lifted fixed pattern "
+              ^Syntax.string_of_term ctxt3 pat_fxd_vard_lifted
+              ^"\nin frozen constraints\n"
+              ^commas (constraints |> map (fst #> MetaRec.norm_with_env_in_run_state ctxt3 #> freeze
+                 #> Syntax.string_of_term ctxt3))
+              ^"\nthat are prepared for non-rotative matching as follows\n"
+              ^commas (constraints |> map (fst #> prep_match false #> Syntax.string_of_term ctxt3))
+              ^"\nand for rotative matching as follows\n"
+              ^commas (constraints |> map (fst #> prep_match true #> Syntax.string_of_term ctxt3))) *)
           in
-            case get_first (fn (C, _) => MetaRec.pattern_match_envctxt ctxt3 (pat_fxd_vard, freeze C)) constraints of
-              SOME ctxt4 =>
+            (* FIXME: if pattern conclusion head is a parameter itself, matching modulo parameter rotation
+              makes no sense. We remove matching modulo parameter rotation for now, as there is no use
+              case anymore with on-the-fly contextual discharge of constraints. *)
+            case
+              (* TODO(opt): matching without local_free rotation first might not be performance gain after all,
+                 because the real processing only starts in result function *)
+              (* NB: in the mod_param_rot case, the metaex-quantified variables became unlifted unifvars
+                 and the unifvars for the fixes are unlifted as well, so pat_fxd_vard_fixvard is a pattern *)
+              get_first (fn ((C, _), mod_param_rot) =>
+                  let
+                    val pat' = if mod_param_rot then pat_fxd_vard_fixvard else pat_fxd_vard_lifted
+                    val C' = prep_match mod_param_rot C
+                  in
+                    case MetaRec.pattern_match_envctxt ctxt3 (pat', C') of
+                      NONE => NONE
+                    | SOME ctxt4 =>
+                        (*if fix_vars |> exists (fn x1 => fix_vars |> exists (fn x2 =>
+                             x1 <> x2 andalso
+                             ((x1, x2) |> pairself (MetaRec.norm_with_env_in_run_state ctxt4)
+                             |> (op aconv))))
+                        then (* discovered local_free "permutation" is not injective *)
+                          NONE
+                        else *)
+                         let
+                           (* NB: in mod_param_rot case we only want to ensure existence of match against
+                             pattern modulo fixes permutation.
+                             Actual permutation is calculated in result function.
+                             This is why we norm pat_fxd_vard instead of pat_fxd_vard_fixvard. *)
+                           val pat_inst = (if mod_param_rot then pat_fxd_vard else pat_fxd_liftvard)
+                             |> MetaRec.norm_with_env_in_run_state ctxt4 |> thaw
+                           val C_normed = C |> MetaRec.norm_with_env_in_run_state ctxt4
+
+                           (*val _ = 
+                             let 
+                               val envdiff = MetaRec.get_the_env_in_run_state ctxt4 |> Envir.term_env |> Vartab.dest
+                                 |> subtract (pairself fst #> (op =))
+                                      (MetaRec.get_the_env_in_run_state ctxt3 |> Envir.term_env  |> Vartab.dest)
+                             in 
+                               tracing ("ex_constraint_proc: found constraint "
+                                 ^Syntax.string_of_term ctxt4 pat_inst
+                                 (*^"\n  (= "^Syntax.string_of_term ctxt4 C_normed^")" *)
+                                 ^"\nmatching pattern "^Syntax.string_of_term ctxt4 pat
+                                 (*^"\n  (pat_fxd_liftvard = "^Syntax.string_of_term ctxt4 pat_fxd_liftvard
+                                 ^"\n  ,instantiated pat_fxd_liftvard = "^MetaRec.str_of_normed_term ctxt4 pat_fxd_liftvard
+                                 ^"\n  ,instantiated and thawed pat_fxd_liftvard = "
+                                   ^Syntax.string_of_term ctxt4
+                                     (MetaRec.norm_with_env_in_run_state ctxt4 pat_fxd_liftvard |> thaw)^")"
+                                 ^"\nactual preparation: "^commas ([pat', C'] |> map (Syntax.string_of_term ctxt4))
+                                 ^"\nterm instantiation from match:\n  "
+                                 ^commas (envdiff |> map (fn (ixn, (T, t)) =>
+                                    Syntax.string_of_term ctxt4 (Var(ixn,T)) ^ " := "
+                                      ^MetaRec.str_of_normed_term ctxt4 t)) *))
+                             end *)
+                         in
+                           SOME ((pat_inst, C_normed), ctxt4)
+                         end
+                  end)
+                (map (rpair false) constraints (* @ map (rpair true) constraints *))
+            of
+              SOME ((pat_inst, C), ctxt4) =>
                 let
-                  val pat_inst = MetaRec.norm_with_env_in_run_state ctxt4 pat_fxd_vard |> thaw
-
-                  (* val _ = tracing ("ex_constraint_proc: found constraint "
-                    ^Syntax.string_of_term ctxt4 pat_inst
-                    ^" matching pattern "^Syntax.string_of_term ctxt4 pat) *)
-
+                  val { fix_necessary_tab, constraint_to_pats, ...} = ExConstraintMemoization.get linctxt
                   val memo_net2 = memo_net |> Net.insert_term (eq_fst (aconv_norm ctxt4))
-                    (pat_indexing, (pat, pat_inst))
+                    (pat_indexing, (pat, (pat_inst, C)))
+                  val constraint_to_pats2 = constraint_to_pats
+                    |> Net.insert_term_safe (eq_pair (aconv_norm ctxt4) (aconv_norm ctxt4))
+                      (Envir.eta_contract C, (C, pat)) 
+                  val fix_necessary_tab2 = fix_necessary_tab |> fold (fn fix =>
+                      Symtab.cons_list (fst (Term.dest_Free fix), pat)) 
+                    local_frees
                   val ctxt5 = ctxt4 |> MetaRec.map_linear_ctxt_in_run_state
-                    (K (linctxt |> ExConstraintMemoization.map (K memo_net2)))
+                    (K (linctxt |> ExConstraintMemoization.map (K
+                      {memo_net=memo_net2, constraint_to_pats=constraint_to_pats2,
+                        fix_necessary_tab=fix_necessary_tab2})))
                 in
-                  result pat_inst ctxt5
+                  result pat_inst C ctxt5
                 end
-            | NONE => fail_cont ctxt3 ("no constraint matching "
-                ^Syntax.string_of_term ctxt3 pat_fxd_vard^" found")
+            | NONE =>
+                let
+                  val msg = ("ex_constraint_proc: no constraint matching "
+                    ^Syntax.string_of_term ctxt3 pat^" found")
+                  (* val _ = tracing msg *)
+                in
+                  fail_cont ctxt3 msg
+                end
           end
+    end
+
     end
 *}
 
